theories/Core/KTreeFacts.v
@@ -1,0 +1,1067 @@
+(* begin hide *)
+From Coq Require Import
+     Morphisms.
+
+From Paco Require Import paco.
+
+From ITree Require Import
+     Basics.Basics
+     Basics.Functions
+     Core.ITree
+     Core.KTree
+     Eq.UpToTaus
+     Eq.SimUpToTaus
+     Indexed.OpenSum.
+
+Import ITreeNotations.
+Local Open Scope itree_scope.
+(* end hide *)
+
+(* Facts about [loop] *)
+
+Notation loop_once_ f loop_ :=
+  (loop_once f (fun cb => Tau (loop_ f%function cb))).
+
+Lemma unfold_loop'' {E A B C} (f : C + A -> itree E (C + B)) (x : C + A) :
+    observe (loop_ f x)
+  = observe (loop_once f (fun cb => Tau (loop_ f cb)) x).
+Proof. reflexivity. Qed.
+
+Lemma unfold_loop' {E A B C} (f : C + A -> itree E (C + B)) (x : C + A) :
+    loop_ f x
+  ≅ loop_once f (fun cb => Tau (loop_ f cb)) x.
+Proof.
+  rewrite itree_eta, (itree_eta (loop_once _ _ _)).
+  reflexivity.
+Qed.
+
+Lemma unfold_loop {E A B C} (f : C + A -> itree E (C + B)) (x : C + A) :
+    loop_ f x
+  ≈ loop_once f (loop_ f) x.
+Proof.
+  rewrite unfold_loop'.
+  apply eutt_bind; try reflexivity.
+  intros []; try reflexivity.
+  rewrite tau_eutt; reflexivity.
+Qed.
+
+(* Equations for a traced monoidal category *)
+
+Lemma loop_natural_l {E A A' B C} (f : A -> itree E A')
+      (body : C + A' -> itree E (C + B)) (a : A) :
+    ITree.bind (f a) (loop body)
+  ≅ loop (fun ca =>
+      match ca with
+      | inl c => Ret (inl c)
+      | inr a => ITree.map inr (f a)
+      end >>= body) a.
+Proof.
+  unfold loop.
+  rewrite unfold_loop'; unfold loop_once.
+  unfold ITree.map. autorewrite with itree.
+  eapply eq_itree_bind; try reflexivity.
+  intros a' _ []. autorewrite with itree.
+  remember (inr a') as ca eqn:EQ; clear EQ a'.
+  pupto2_init. revert ca; clear; pcofix self; intro ca.
+  rewrite unfold_loop'; unfold loop_once.
+  pupto2 @eq_itree_clo_bind; econstructor; try reflexivity.
+  intros [c | b]; intros; subst.
+  - match goal with
+    | [ |- _ _ (Tau (loop_ ?f _)) ] => rewrite (unfold_loop' f)
+    end.
+    unfold loop_once_.
+    rewrite ret_bind_. (* TODO: [ret_bind] doesn't work. *)
+    pfold; constructor; auto.
+  - pfold; constructor; auto.
+Qed.
+
+Lemma loop_natural_r {E A B B' C} (f : B -> itree E B')
+      (body : C + A -> itree E (C + B)) (a : A) :
+    loop body a >>= f
+  ≅ loop (fun ca => body ca >>= fun cb =>
+      match cb with
+      | inl c => Ret (inl c)
+      | inr b => ITree.map inr (f b)
+      end) a.
+Proof.
+  unfold loop.
+  remember (inr a) as ca eqn:EQ; clear EQ a.
+  pupto2_init. revert ca; clear; pcofix self; intro ca.
+  rewrite !unfold_loop'; unfold loop_once.
+  rewrite !bind_bind.
+  pupto2 @eq_itree_clo_bind; econstructor; try reflexivity.
+  intros [c | b]; intros; subst.
+  - rewrite ret_bind_, tau_bind_.
+    pfold; constructor; auto.
+  - autorewrite with itree.
+    pupto2_final; apply reflexivity.
+Qed.
+
+Lemma loop_dinatural {E A B C C'} (f : C -> itree E C')
+      (body : C' + A -> itree E (C + B)) (a : A) :
+    loop (fun c'a => body c'a >>= fun cb =>
+      match cb with
+      | inl c => Tau (ITree.map inl (f c))
+      | inr b => Ret (inr b)
+      end) a
+  ≅ loop (fun ca =>
+      match ca with
+      | inl c => f c >>= fun c' => Tau (Ret (inl c'))
+      | inr a => Ret (inr a)
+      end >>= body) a.
+Proof.
+  unfold loop.
+  do 2 rewrite unfold_loop'; unfold loop_once.
+  autorewrite with itree.
+  eapply eq_itree_bind; try reflexivity.
+  clear a; intros cb _ [].
+  pupto2_init. revert cb; pcofix self; intros.
+  destruct cb as [c | b].
+  - rewrite tau_bind.
+    pfold; constructor; pupto2_final; left.
+    rewrite map_bind.
+    rewrite (unfold_loop' _ (inl c)); unfold loop_once.
+    autorewrite with itree.
+    pupto2 eq_itree_clo_bind; econstructor; try reflexivity.
+    intros c'; intros; subst.
+    rewrite tau_bind.
+    rewrite ret_bind_.
+    rewrite unfold_loop'; unfold loop_once.
+    rewrite bind_bind.
+    pfold; constructor.
+    pupto2 eq_itree_clo_bind; econstructor; try reflexivity.
+    intros; subst. eauto.
+  - rewrite ret_bind.
+    pupto2_final; apply reflexivity.
+Qed.
+
+Lemma vanishing1 {E A B} (f : Empty_set + A -> itree E (Empty_set + B))
+      (a : A) :
+  loop f a ≅ ITree.map sum_empty_l (f (inr a)).
+Proof.
+  unfold loop.
+  rewrite unfold_loop'; unfold loop_once, ITree.map.
+  eapply eq_itree_bind; try reflexivity.
+  intros [[]| b] _ []; reflexivity.
+Qed.
+
+Lemma vanishing2 {E A B C D} (f : D + (C + A) -> itree E (D + (C + B)))
+      (a : A) :
+    loop (loop f) a
+  ≅ loop (fun dca => ITree.map sum_assoc_l (f (sum_assoc_r dca))) a.
+Proof.
+  unfold loop; rewrite 2 unfold_loop'; unfold loop_once.
+  rewrite map_bind.
+  rewrite unfold_loop'; unfold loop_once.
+  rewrite bind_bind.
+  eapply eq_itree_bind; try reflexivity.
+  clear a; intros dcb _ [].
+  pupto2_init. revert dcb; pcofix self; intros.
+  destruct dcb as [d | [c | b]]; simpl.
+  - (* d *)
+    rewrite tau_bind.
+    rewrite 2 unfold_loop'; unfold loop_once.
+    autorewrite with itree.
+    pfold; constructor.
+    pupto2 eq_itree_clo_bind; econstructor; try reflexivity.
+    intros; subst. auto.
+  - (* c *)
+    rewrite ret_bind.
+    rewrite 2 unfold_loop'; unfold loop_once.
+    rewrite unfold_loop'; unfold loop_once.
+    autorewrite with itree.
+    pfold; constructor.
+    pupto2 eq_itree_clo_bind; econstructor; try reflexivity.
+    intros; subst. auto.
+  - (* b *)
+    rewrite ret_bind.
+    pupto2_final; apply reflexivity.
+Qed.
+
+Lemma superposing1 {E A B C D D'} (f : C + A -> itree E (C + B))
+      (g : D -> itree E D') (a : A) :
+    ITree.map inl (loop f a)
+  ≅ loop (fun cad =>
+      match cad with
+      | inl c => ITree.map (sum_bimap id inl) (f (inl c))
+      | inr (inl a) => ITree.map (sum_bimap id inl) (f (inr a))
+      | inr (inr d) => ITree.map (inr ∘ inr) (g d)
+      end) (inl a).
+Proof.
+  unfold loop.
+  remember (inr a) as inra eqn:Hr.
+  remember (inr (inl a)) as inla eqn:Hl.
+  assert (Hlr : match inra with
+                | inl c => inl c
+                | inr a => inr (inl a)
+                end = inla).
+  { subst; auto. }
+  clear a Hl Hr.
+  unfold ITree.map.
+  pupto2_init. revert inla inra Hlr; pcofix self; intros.
+  rewrite 2 unfold_loop'; unfold loop_once.
+  rewrite bind_bind.
+  destruct inra as [c | a]; subst.
+  - rewrite bind_bind; setoid_rewrite ret_bind_.
+    pupto2 eq_itree_clo_bind; econstructor; try reflexivity.
+    intros [c' | b]; simpl; intros; subst.
+    + rewrite tau_bind. pfold; constructor.
+      pupto2_final. auto.
+    + rewrite ret_bind. pupto2_final; apply reflexivity.
+  - rewrite bind_bind; setoid_rewrite ret_bind_.
+    pupto2 eq_itree_clo_bind; econstructor; try reflexivity.
+    intros [c' | b]; simpl; intros; subst.
+    + rewrite tau_bind. pfold; constructor.
+      pupto2_final. auto.
+    + rewrite ret_bind_. pupto2_final; apply reflexivity.
+Qed.
+
+Lemma superposing2 {E A B C D D'} (f : C + A -> itree E (C + B))
+      (g : D -> itree E D') (d : D) :
+    ITree.map inr (g d)
+  ≅ loop (fun cad =>
+      match cad with
+      | inl c => ITree.map (sum_bimap id inl) (f (inl c))
+      | inr (inl a) => ITree.map (sum_bimap id inl) (f (inr a))
+      | inr (inr d) => ITree.map (inr ∘ inr) (g d)
+      end) (inr d).
+Proof.
+  unfold loop; rewrite unfold_loop'; unfold loop_once.
+  rewrite map_bind; unfold ITree.map.
+  eapply eq_itree_bind; try reflexivity.
+  intros d' _ []. reflexivity.
+Qed.
+
+Lemma yanking {E A} (a : A) :
+  @loop E _ _ _ (fun aa => Ret (sum_comm aa)) a ≅ Tau (Ret a).
+Proof.
+  rewrite itree_eta; cbn; apply eq_itree_tau.
+  rewrite itree_eta; reflexivity.
+Qed.
+
+Definition sum_map1 {A B C} (f : A -> B) (ac : A + C) : B + C :=
+  match ac with
+  | inl a => inl (f a)
+  | inr c => inr c
+  end.
+
+Instance eq_itree_loop {E A B C} :
+  Proper ((eq ==> eq_itree eq) ==> eq ==> eq_itree eq) (@loop E A B C).
+Proof.
+  repeat intro; subst.
+  unfold loop.
+  remember (inr _) as ca eqn:EQ; clear EQ y0.
+  pupto2_init. revert ca; pcofix self; intros.
+  rewrite 2 unfold_loop'; unfold loop_once.
+  pupto2 eq_itree_clo_bind; econstructor; try auto.
+  intros [c | b]; intros; subst; pfold; constructor; auto.
+Qed.
+
+Section eutt_loop.
+
+Context {E : Type -> Type} {A B C : Type}.
+Variables f1 f2 : C + A -> itree E (C + B).
+Hypothesis eutt_f : forall ca, sutt eq (f1 ca) (f2 ca).
+
+Inductive loop_preinv (t1 t2 : itree E B) : Prop :=
+| loop_inv_main ca :
+    t1 ≅ loop_ f1 ca ->
+    t2 ≅ loop_ f2 ca ->
+    loop_preinv t1 t2
+| loop_inv_bind u1 u2 :
+    sutt eq u1 u2 ->
+    t1 ≅ (cb <- u1;;
+       match cb with
+       | inl c => Tau (loop_ f1 (inl c))
+       | inr b => Ret b
+       end) ->
+    t2 ≅ (cb <- u2;;
+       match cb with
+       | inl c => Tau (loop_ f2 (inl c))
+       | inr b => Ret b
+       end) ->
+    loop_preinv t1 t2
+.
+Hint Constructors loop_preinv.
+
+Lemma eutt_loop_inv_main_step (ca : C + A) t1 t2 :
+  t1 ≅ loop_ f1 ca ->
+  t2 ≅ loop_ f2 ca ->
+  suttF1 eq (going loop_preinv) (observe t1) (observe t2).
+Proof.
+  intros H1 H2.
+  rewrite unfold_loop' in H1.
+  rewrite unfold_loop' in H2.
+  unfold loop_once.
+  specialize (eutt_f ca).
+  apply sutt_is_sutt1 in eutt_f.
+  punfold eutt_f.
+  unfold loop_once in H1.
+  unfold loop_once in H2.
+  rewrite unfold_bind in H1.
+  rewrite unfold_bind in H2.
+
+  revert t1 t2 H1 H2.
+  induction eutt_f; intros z1 z2 H1 H2.
+
+  - subst; destruct r2.
+    + apply eq_itree_tau_inv1 in H1.
+      destruct H1 as [t1' [Ht1 Ht1']].
+      apply eq_itree_tau_inv1 in H2.
+      destruct H2 as [t2' [Ht2 Ht2']].
+      rewrite Ht1, Ht2.
+      repeat constructor.
+      econstructor; try rewrite <- itree_eta; eassumption.
+    + apply eq_itree_ret_inv1 in H1.
+      apply eq_itree_ret_inv1 in H2.
+      rewrite H1, H2.
+      auto.
+
+  - pclearbot. apply eq_itree_vis_inv1 in H1.
+    apply eq_itree_vis_inv1 in H2.
+    destruct H1 as [k01 [Hk1 Hk1']].
+    destruct H2 as [k02 [Hk2 Hk2']].
+    rewrite Hk1, Hk2.
+    constructor; intros.
+    repeat constructor.
+    eapply loop_inv_bind.
+    + apply sutt_is_sutt1, SUTTK.
+    + rewrite <- itree_eta; auto.
+    + rewrite <- itree_eta; auto.
+
+  - apply eq_itree_tau_inv1 in H2.
+    destruct H2 as [t2' [Ht2 Ht2']].
+    rewrite Ht2.
+    constructor.
+    apply IHs; auto. rewrite <- unfold_bind; auto.
+
+  - pclearbot.
+    replace ot2 with (observe (go ot2)) in *.
+    rewrite <- unfold_bind in H2.
+    apply eq_itree_tau_inv1 in H1.
+    destruct H1 as [t1' [Ht1 Ht1']].
+    rewrite Ht1.
+    repeat constructor.
+    eapply loop_inv_bind.
+    + apply sutt_is_sutt1. eauto.
+    + rewrite <- itree_eta; auto.
+    + rewrite <- itree_eta; auto.
+    + auto.
+Qed.
+
+Lemma eutt_loop_inv ot1 ot2 :
+  loop_preinv (go ot1) (go ot2) -> paco2 (suttF1 eq) bot2 ot1 ot2.
+Proof.
+  intros HH.
+  revert ot1 ot2 HH; pcofix self; intros. pfold.
+  destruct HH as [ca H1 H2 | u1 u2 Hu H1 H2].
+  - eapply monotone_suttF1.
+    + eapply (eutt_loop_inv_main_step ca (go ot1) (go ot2)); eauto.
+    + intros ? ? []. right. eapply self; eauto.
+  - apply sutt_is_sutt1 in Hu.
+    punfold Hu.
+    rewrite unfold_bind in H1.
+    rewrite unfold_bind in H2.
+    revert ot1 ot2 H1 H2; induction Hu; intros.
+
+    + subst; destruct r2.
+      * apply eq_itree_tau_inv1 in H1.
+        apply eq_itree_tau_inv1 in H2.
+        simpl in H1, H2.
+        destruct H1 as [? []], H2 as [? []].
+        subst.
+        do 2 constructor. right.
+        apply self.
+        eapply loop_inv_main; rewrite <- itree_eta; eauto.
+      * apply eq_itree_ret_inv1 in H1.
+        apply eq_itree_ret_inv1 in H2.
+        simpl in H1, H2. subst; auto.
+
+    + pclearbot.
+      apply eq_itree_vis_inv1 in H1.
+      apply eq_itree_vis_inv1 in H2.
+      simpl in H1, H2.
+      destruct H1 as [? []], H2 as [? []].
+      subst; constructor.
+      right. apply self.
+      eapply loop_inv_bind.
+      * apply sutt_is_sutt1. eapply SUTTK.
+      * rewrite <- itree_eta; auto.
+      * rewrite <- itree_eta; auto.
+
+    + apply eq_itree_tau_inv1 in H2.
+      simpl in H2.
+      destruct H2 as [t2' [Ht2 Ht2']].
+      rewrite Ht2.
+      constructor.
+      apply IHHu; auto.
+      rewrite <- itree_eta, <- unfold_bind; auto.
+
+    + pclearbot.
+      replace ot2 with (observe (go ot2)) in *.
+      rewrite <- unfold_bind in H2.
+      apply eq_itree_tau_inv1 in H1.
+      simpl in H1.
+      destruct H1 as [t1' [Ht1 Ht1']].
+      rewrite Ht1.
+      constructor.
+      right; apply self.
+      eapply loop_inv_bind.
+      * apply sutt_is_sutt1.
+        eapply EQTAUS.
+      * rewrite <- itree_eta; auto.
+      * auto.
+      * auto.
+Qed.
+
+End eutt_loop.
+
+Instance sutt_loop {E A B C} :
+  Proper (pointwise_relation _ (sutt eq) ==> eq ==> sutt eq) (@loop E A B C).
+Proof.
+  repeat intro; subst. apply sutt_is_sutt1.
+
+  eapply eutt_loop_inv.
+  - eauto.
+  - unfold loop; econstructor; rewrite <- itree_eta; reflexivity.
+Qed.
+
+Instance eutt_loop {E A B C} :
+  Proper (pointwise_relation _ (eutt eq) ==> eq ==> eutt eq) (@loop E A B C).
+Proof.
+  repeat intro; subst.
+  repeat red in H.
+  eapply sutt_eutt.
+  - eapply sutt_loop; auto.
+    repeat intro; subst.
+    apply eutt_sutt; auto.
+  - eapply paco2_mon_gen.
+    + eapply sutt_loop; auto.
+      repeat intro.
+      apply eutt_sutt. apply symmetry; auto.
+    + intros. eapply monotone_sutt_RR; try eassumption.
+      red; auto.
+    + auto.
+Qed.
+
+(** ** Equations *)
+
+Section CategoryLaws.
+
+Context {E : Type -> Type}.
+
+(** *** [compose_ktree] respect eq_ktree *)
+Global Instance eq_ktree_compose {A B C} :
+  Proper (eq_ktree ==> eq_ktree ==> eq_ktree) (@ITree.cat E A B C).
+Proof.
+  intros ab ab' eqAB bc bc' eqBC.
+  intro a.
+  unfold ITree.cat.
+  rewrite (eqAB a).
+  apply eutt_bind; try reflexivity.
+  intro b; rewrite (eqBC b); reflexivity.
+Qed.
+
+(** *** [compose_ktree] is associative *)
+Lemma compose_ktree_assoc {A B C D}
+      (ab : ktree E A B) (bc : ktree E B C) (cd : ktree E C D) :
+  ((ab >=> bc) >=> cd) ⩯ (ab >=> (bc >=> cd)).
+Proof.
+  intros a.
+  unfold ITree.cat.
+  rewrite bind_bind.
+  apply eutt_bind; try reflexivity.
+Qed.
+
+(** *** [id_ktree] respect identity laws *)
+Lemma id_ktree_left {A B}: forall (f: ktree E A B),
+    id_ktree >=> f ⩯ f.
+Proof.
+  intros f a; unfold ITree.cat, id_ktree.
+  rewrite itree_eta; rewrite ret_bind. rewrite <- itree_eta; reflexivity.
+Qed.
+
+Lemma id_ktree_right {A B}: forall (f: ktree E A B),
+    f >=> id_ktree ⩯ f.
+Proof.
+  intros f a; unfold ITree.cat, id_ktree.
+  rewrite <- (bind_ret (f a)) at 2.
+  reflexivity.
+Qed.
+
+End CategoryLaws.
+
+(** *** [lift] properties *)
+
+Section LiftLaws.
+
+Context {E : Type -> Type}.
+
+(** *** [lift_ktree] is well-behaved *)
+
+Global Instance eq_lift_ktree {A B} :
+  Proper (eeq ==> eq_ktree) (@lift_ktree E A B).
+Proof.
+  repeat intro.
+  unfold lift_ktree.
+  erewrite (H a); reflexivity.
+Qed.
+
+Lemma lift_ktree_id {A: Type}: @id_ktree E A ⩯ lift_ktree id.
+Proof.
+  unfold id_ktree, lift_ktree; reflexivity.
+Qed.
+
+Fact compose_lift_ktree {A B C} (ab : A -> B) (bc : B -> C) :
+  (@lift_ktree E _ _ ab >=> lift_ktree bc) ⩯ (lift_ktree (bc ∘ ab)).
+Proof.
+  intros a.
+  unfold lift_ktree, ITree.cat.
+  rewrite ret_bind_.
+  reflexivity.
+Qed.
+
+Fact compose_lift_ktree_l {A B C D} (f: A -> B) (g: B -> C) (k: ktree E C D) :
+  (lift_ktree f >=> (lift_ktree g >=> k)) ⩯ (lift_ktree (g ∘ f) >=> k).
+Proof.
+  rewrite <- compose_ktree_assoc.
+  rewrite compose_lift_ktree.
+  reflexivity.
+Qed.
+
+Fact compose_lift_ktree_r {A B C D} (f: B -> C) (g: C -> D) (k: ktree E A B) :
+  ((k >=> lift_ktree f) >=> lift_ktree g) ⩯ (k >=> lift_ktree (g ∘ f)).
+Proof.
+  rewrite compose_ktree_assoc.
+  rewrite compose_lift_ktree.
+  reflexivity.
+Qed.
+
+Fact lift_compose_ktree {A B C}: forall (f:A -> B) (bc: ktree E B C),
+    lift_ktree f >=> bc ⩯ fun a => bc (f a).
+Proof.
+  intros; intro a.
+  unfold lift_ktree, ITree.cat.
+  rewrite ret_bind_. reflexivity.
+Qed.
+
+Fact compose_ktree_lift {A B C}: forall (ab: ktree E A B) (g:B -> C),
+    eq_ktree (ab >=> lift_ktree g)
+             (fun a => ITree.map g (ab a)).
+Proof.
+  intros; intro a.
+  unfold ITree.map.
+  apply eutt_bind.
+  reflexivity.
+  intro; reflexivity.
+Qed.
+
+Lemma sym_ktree_unfold {A B}:
+  lift_ktree sum_comm ⩯ @sym_ktree E A B.
+Proof.
+  reflexivity.
+Qed.
+
+End LiftLaws.
+
+Section MonoidalCategoryLaws.
+
+Context {E : Type -> Type}.
+
+(** *** [associators]  *)
+Lemma assoc_lr {A B C} :
+  @assoc_ktree_l E A B C >=> assoc_ktree_r ⩯ id_ktree.
+Proof.
+  unfold assoc_ktree_l, assoc_ktree_r.
+  rewrite compose_lift_ktree.
+  intros [| []]; reflexivity.
+Qed.
+
+Lemma assoc_rl {A B C} :
+  @assoc_ktree_r E A B C >=> assoc_ktree_l ⩯ id_ktree.
+Proof.
+  unfold assoc_ktree_l, assoc_ktree_r.
+  rewrite compose_lift_ktree.
+  intros [[]|]; reflexivity.
+Qed.
+
+(** *** [sum_elim] lemmas *)
+
+Fact compose_sum_elim {A B C D} (ac : ktree E A C) (bc : ktree E B C) (cd : ktree E C D) :
+  sum_elim ac bc >=> cd ⩯ sum_elim (ac >=> cd) (bc >=> cd).
+Proof.
+  intros; intros [];
+    (unfold ITree.map; simpl; apply eutt_bind; reflexivity).
+Qed.
+
+Fact lift_sum_elim {A B C} (ac : A -> C) (bc : B -> C) :
+    sum_elim (@lift_ktree E _ _ ac) (lift_ktree bc)
+  ⩯ lift_ktree (sum_elim ac bc).
+Proof.
+  intros []; reflexivity.
+Qed.
+
+(** *** [Unitors] lemmas *)
+
+(* TODO: replacing l by λ breaks PG (retracts like crazy, or if you go too far it can't retract at all from the second lemma) (ρ is fine, interestingly) *)
+Lemma elim_l_ktree {A B: Type} (ab: @ktree E A (I + B)) :
+  ab >=> λ_ktree ⩯ (fun a: A => ITree.map sum_empty_l (ab a)).
+Proof.
+  intros; apply compose_ktree_lift.
+Qed.
+
+Lemma elim_l_ktree' {A B: Type} (f: @ktree E (I + A) (I + B)) :
+  λ_ktree' >=> f ⩯ fun a => f (inr a).
+Proof.
+  repeat intro.
+  unfold λ_ktree', ITree.cat, lift_ktree.
+  rewrite ret_bind_; reflexivity.
+Qed.
+
+Lemma elim_ρ_ktree' {A B: Type} (f: @ktree E (A + I) (B + I)) :
+  ρ_ktree' >=> f ⩯ fun a => f (inl a).
+Proof.
+  repeat intro.
+  unfold ρ_ktree', ITree.cat, lift_ktree.
+  rewrite ret_bind_; reflexivity.
+Qed.
+
+Lemma elim_ρ_ktree {A B: Type} (ab: @ktree E A (B + I)) :
+  ab >=> ρ_ktree ⩯ (fun a: A => ITree.map sum_empty_r (ab a)).
+Proof.
+  intros; apply compose_ktree_lift.
+Qed.
+
+(** *** [tensor] lemmas *)
+
+Global Instance eq_ktree_tensor {A B C D}:
+  Proper (eq_ktree ==> eq_ktree ==> eq_ktree) (@tensor_ktree E A B C D).
+Proof.
+  intros ac ac' eqac bd bd' eqbd.
+  unfold tensor_ktree.
+  rewrite eqac, eqbd; reflexivity.
+Qed.
+
+Fact tensor_id_lift {A B C} (f : B -> C) :
+  (@id_ktree E A) ⊗ (lift_ktree f) ⩯ lift_ktree (sum_bimap id f).
+Proof.
+  unfold tensor_ktree.
+  rewrite compose_lift_ktree, id_ktree_left.
+  rewrite lift_sum_elim.
+  reflexivity.
+Qed.
+
+Fact tensor_lift_id {A B C} (f : A -> B) :
+  (lift_ktree f) ⊗ (@id_ktree E C) ⩯ lift_ktree (sum_bimap f id).
+Proof.
+  unfold tensor_ktree.
+  rewrite compose_lift_ktree, id_ktree_left.
+  rewrite lift_sum_elim.
+  reflexivity.
+Qed.
+
+Lemma tensor_id {A B} :
+  id_ktree ⊗ id_ktree ⩯ @id_ktree E (A + B).
+Proof.
+  unfold tensor_ktree, ITree.cat, id_ktree.
+  intros []; cbn; rewrite ret_bind_; reflexivity.
+Qed.
+
+Lemma assoc_I {A B}:
+  @assoc_ktree_r E A I B >=> id_ktree ⊗ λ_ktree ⩯ ρ_ktree ⊗ id_ktree.
+Proof.
+  unfold ρ_ktree,λ_ktree.
+  rewrite tensor_lift_id, tensor_id_lift.
+  unfold assoc_ktree_r.
+  rewrite compose_lift_ktree.
+  apply eq_lift_ktree.
+  intros [[|]|]; compute; try reflexivity.
+  destruct i.
+Qed.
+
+Lemma cat_tensor {A1 A2 A3 B1 B2 B3}
+      (f1 : ktree E A1 A2) (f2 : ktree E A2 A3)
+      (g1 : ktree E B1 B2) (g2 : ktree E B2 B3) :
+  (f1 ⊗ g1) >=> (f2 ⊗ g2) ⩯ (f1 >=> f2) ⊗ (g1 >=> g2).
+Proof.
+  unfold tensor_ktree, ITree.cat, lift_ktree; simpl.
+  intros []; simpl;
+    rewrite !bind_bind; setoid_rewrite ret_bind_; reflexivity.
+Qed.
+
+Lemma sum_elim_compose {A B C D F}
+      (ac: ktree E A (C + D)) (bc: ktree E B (C + D))
+      (cf: ktree E C F) (df: ktree E D F) :
+    sum_elim ac bc >=> sum_elim cf df
+  ⩯ sum_elim (ac >=> (sum_elim cf df)) (bc >=> (sum_elim cf df)).
+Proof.
+  intros.
+  unfold ITree.map.
+  intros []; reflexivity.
+Qed.
+
+Lemma inl_sum_elim {A B C} (ac: ktree E A C) (bc: ktree E B C) :
+  lift_ktree inl >=> sum_elim ac bc ⩯ ac.
+Proof.
+  intros.
+  unfold ITree.cat, lift_ktree.
+  intros ?.
+  rewrite ret_bind_.
+  reflexivity.
+Qed.
+
+Lemma inr_sum_elim {A B C} (ac: ktree E A C) (bc: ktree E B C) :
+  lift_ktree inr >=> sum_elim ac bc ⩯ bc.
+Proof.
+  intros.
+  unfold ITree.cat, lift_ktree.
+  intros ?.
+  rewrite ret_bind_.
+  reflexivity.
+Qed.
+
+Lemma tensor_ktree_slide {A B C D} (ac: ktree E A C) (bd: ktree E B D) :
+  ac ⊗ bd ⩯ ac ⊗ id_ktree >=> id_ktree ⊗ bd.
+Proof.
+  intros.
+  unfold tensor_ktree.
+  repeat rewrite id_ktree_left.
+  rewrite sum_elim_compose.
+  rewrite compose_ktree_assoc.
+  rewrite inl_sum_elim, inr_sum_elim.
+  reflexivity.
+Qed.
+
+Lemma assoc_coherent_r {A B C D}:
+    @assoc_ktree_r E A B C ⊗ @id_ktree E D
+      >=> assoc_ktree_r
+      >=> id_ktree ⊗ assoc_ktree_r
+  ⩯ assoc_ktree_r >=> assoc_ktree_r.
+Proof.
+  unfold tensor_ktree, assoc_ktree_r.
+  repeat rewrite id_ktree_left.
+  repeat rewrite compose_sum_elim.
+  repeat rewrite compose_lift_ktree.
+  rewrite lift_sum_elim.
+  repeat rewrite compose_lift_ktree.
+  rewrite lift_sum_elim.
+  apply eq_lift_ktree.
+  intros [[[|]|]|]; reflexivity.
+Qed.
+
+Lemma assoc_coherent_l {A B C D}:
+    @id_ktree E A ⊗ @assoc_ktree_l E B C D
+      >=> assoc_ktree_l
+      >=> assoc_ktree_l ⊗ id_ktree
+  ⩯ assoc_ktree_l >=> assoc_ktree_l.
+Proof.
+  unfold tensor_ktree, assoc_ktree_l.
+  repeat rewrite id_ktree_left.
+  repeat rewrite compose_sum_elim.
+  repeat rewrite compose_lift_ktree.
+  rewrite lift_sum_elim.
+  repeat rewrite compose_lift_ktree.
+  rewrite lift_sum_elim.
+  apply eq_lift_ktree.
+  intros [|[|[|]]]; reflexivity.
+Qed.
+
+(** *** [sym] lemmas *)
+
+Lemma sym_unit_ktree {A} :
+  sym_ktree >=> λ_ktree ⩯ @ρ_ktree E A.
+Proof.
+  unfold sym_ktree, ρ_ktree, λ_ktree.
+  rewrite lift_compose_ktree.
+  intros []; simpl; reflexivity.
+Qed.
+
+Lemma sym_assoc_ktree {A B C}:
+    @assoc_ktree_r E A B C >=> sym_ktree >=> assoc_ktree_r
+  ⩯ (sym_ktree ⊗ id_ktree) >=> assoc_ktree_r >=> (id_ktree ⊗ sym_ktree).
+Proof.
+  unfold assoc_ktree_r, sym_ktree.
+  rewrite tensor_lift_id, tensor_id_lift.
+  repeat rewrite compose_lift_ktree.
+  apply eq_lift_ktree.
+  intros [[|]|]; compute; reflexivity.
+Qed.
+
+Lemma sym_nilpotent {A B: Type}:
+  sym_ktree >=> sym_ktree ⩯ @id_ktree E (A + B).
+Proof.
+  unfold sym_ktree, id_ktree.
+  rewrite compose_lift_ktree.
+  unfold compose.
+  unfold lift_ktree; intros a.
+  setoid_rewrite iso_ff'; reflexivity.
+Qed.
+
+Lemma tensor_swap {A B C D} (ab : ktree E A B) (cd : ktree E C D) :
+  ab ⊗ cd ⩯ (sym_ktree >=> cd ⊗ ab >=> sym_ktree).
+Proof.
+  unfold tensor_ktree.
+  unfold sym_ktree.
+  rewrite !(compose_ktree_lift cd), !(compose_ktree_lift ab), !lift_compose_ktree, !compose_ktree_lift.
+  intros []; cbn; rewrite map_map; cbn;
+    apply eutt_map; try intros []; reflexivity.
+Qed.
+
+End MonoidalCategoryLaws.
+
+(** *** Traced monoidal categories *)
+
+Section TraceLaws.
+
+Context {E : Type -> Type}.
+
+(** *** [loop] lemmas *)
+
+Global Instance eq_ktree_loop {I A B} :
+  Proper (eq_ktree ==> eq_ktree) (@loop E I A B).
+Proof.
+  repeat intro; apply eutt_loop; auto.
+Qed.
+
+(* Naturality of (loop_ktree I A B) in A *)
+(* Or more diagrammatically:
+[[
+        +-----+
+        | ### |
+        +-###-+I
+A----B----###----C
+          ###
+
+is equivalent to:
+
+   +----------+
+   |      ### |
+   +------###-+I
+A----B----###----C
+          ###
+
+]]
+ *)
+
+Lemma compose_loop {I A B C}
+      (bc_: ktree E (I + B) (I + C)) (ab: ktree E A B) :
+    loop ((id_ktree ⊗ ab) >=> bc_)
+  ⩯ ab >=> loop bc_.
+Proof.
+  intros a.
+  rewrite (loop_natural_l ab bc_ a).
+  apply eutt_loop; [intros [] | reflexivity].
+  all: unfold tensor_ktree, sym_ktree, ITree.cat, assoc_ktree_l, assoc_ktree_r, id_ktree, lift_ktree; simpl.
+  - rewrite bind_bind, ret_bind_; reflexivity.
+  - rewrite bind_bind, map_bind.
+    setoid_rewrite ret_bind_; reflexivity.
+Qed.
+
+(* Naturality of (loop I A B) in B *)
+(* Or more diagrammatically:
+[[
+   +-----+
+   | ### |
+   +-###-+I
+A----###----B----C
+     ###
+
+is equivalent to:
+
+   +----------+
+   | ###      |
+   +-###------+I
+A----###----B----C
+     ###
+
+]]
+ *)
+
+Lemma loop_compose {I A B B'}
+      (ab_: ktree E (I + A) (I + B)) (bc: ktree E B B') :
+    loop (ab_ >=> (id_ktree ⊗ bc))
+  ⩯ loop ab_ >=> bc.
+Proof.
+  intros a.
+  rewrite (loop_natural_r bc ab_ a).
+  apply eutt_loop; [intros [] | reflexivity].
+  all: unfold tensor_ktree, sym_ktree, ITree.cat, assoc_ktree_l, assoc_ktree_r, id_ktree, lift_ktree; simpl.
+  - apply eutt_bind; [reflexivity | intros []; simpl].
+    rewrite ret_bind_; reflexivity.
+    reflexivity.
+  - apply eutt_bind; [reflexivity | intros []; simpl].
+    rewrite ret_bind_; reflexivity.
+    reflexivity.
+Qed.
+
+(* Dinaturality of (loop I A B) in I *)
+
+Lemma loop_rename_internal {I J A B}
+      (ab_: ktree E (I + A) (J + B)) (ji: ktree E J I) :
+    loop (ab_ >=> (ji ⊗ id_ktree))
+  ⩯ loop ((ji ⊗ id_ktree) >=> ab_).
+Proof.
+  unfold tensor_ktree, ITree.cat, lift_ktree, sum_elim.
+
+  assert (EQ:forall (x: J + B),
+             match x with
+             | inl a => a0 <- ji a;; Ret (inl a0)
+             | inr b => a <- id_ktree b;; Ret (inr a)
+             end ≈
+                 match x with
+                 | inl a => Tau (ITree.map (@inl I B) (ji a))
+                 | inr b => Ret (inr b)
+                 end).
+  {
+    intros [].
+    symmetry; apply tau_eutt.
+    unfold id_ktree.
+    rewrite ret_bind_; reflexivity.
+  }
+  intros ?.
+  setoid_rewrite EQ.
+  rewrite loop_dinatural.
+  apply eutt_loop; [intros [] | reflexivity].
+  all: unfold id_ktree.
+  all: repeat rewrite bind_bind.
+  2: repeat rewrite ret_bind_; reflexivity.
+  apply eutt_bind; [reflexivity | intros ?].
+  apply eutt_bind; [| intros ?; reflexivity].
+  apply tau_eutt.
+Qed.
+
+(* Loop over the empty set can be erased *)
+Lemma vanishing_ktree {A B: Type} (f: ktree E (I + A) (I + B)) :
+  loop f ⩯ λ_ktree' >=> f >=> λ_ktree.
+Proof.
+  intros a.
+  rewrite vanishing1.
+  unfold λ_ktree,λ_ktree'.
+  unfold ITree.cat, ITree.map, lift_ktree.
+  rewrite bind_bind.
+  rewrite ret_bind_.
+  reflexivity.
+Qed.
+
+(* [loop_loop]:
+
+These two loops:
+
+[[
+    +----------+
+    | +-----+  |
+    | | ### |  |
+    | +-###-+I |
+    +---###----+J
+  A-----###-------B
+        ###
+]]
+
+... can be rewired as a single one:
+
+
+[[
+     +-------+
+     |  ###  |
+     +--###--+(I+J)
+     +--###--+
+  A-----###-----B
+        ###
+]]
+
+ *)
+
+Lemma loop_loop {I J A B} (ab__: ktree E (I + (J + A)) (I + (J + B))) :
+    loop (loop ab__)
+  ⩯ loop (assoc_ktree_r >=> ab__ >=> assoc_ktree_l).
+Proof.
+  intros a.
+  rewrite vanishing2.
+  apply eutt_loop; [intros [[]|] | reflexivity].
+  all: unfold ITree.map, ITree.cat, assoc_ktree_r, assoc_ktree_l, lift_ktree; cbn.
+  all: rewrite bind_bind.
+  all: rewrite ret_bind_.
+  all: reflexivity.
+Qed.
+
+Lemma fold_map {R S}:
+  forall (f: R -> S) (t: itree E R),
+    (x <- t;; Ret (f x)) ≅ (ITree.map f t).
+Proof.
+  intros; reflexivity.
+Qed.
+
+Lemma tensor_ktree_loop {I A B C D}
+      (ab : ktree E (I + A) (I + B)) (cd : ktree E C D) :
+    (loop ab) ⊗ cd
+  ⩯ loop (assoc_ktree_l >=> (ab ⊗ cd) >=> assoc_ktree_r).
+Proof.
+  unfold tensor_ktree, ITree.cat, assoc_ktree_l, assoc_ktree_r, lift_ktree, sum_elim.
+  intros []; simpl.
+  all:setoid_rewrite bind_bind.
+  all:setoid_rewrite ret_bind_.
+  all:rewrite fold_map.
+  1:rewrite (@superposing1 E A B I C D).
+  2:rewrite (@superposing2 E A B I C D).
+  all:unfold sum_bimap, ITree.map, sum_assoc_r,sum_elim; cbn.
+  all:apply eutt_loop; [intros [| []]; cbn | reflexivity].
+  all: setoid_rewrite bind_bind.
+  all:setoid_rewrite ret_bind_.
+  all:reflexivity.
+Qed.
+
+Lemma yanking_ktree {A: Type}:
+  loop sym_ktree ⩯ @id_ktree E A.
+Proof.
+  unfold sym_ktree, lift_ktree.
+  intros ?; rewrite yanking.
+  apply tau_eutt.
+Qed.
+
+Lemma loop_rename_internal' {I J A B} (ij : ktree E I J) (ji: ktree E J I)
+      (ab_: @ktree E (I + A) (I + B)) :
+  (ij >=> ji) ⩯ id_ktree ->
+    loop ((ji ⊗ id_ktree) >=> ab_ >=> (ij ⊗ id_ktree))
+  ⩯ loop ab_.
+Proof.
+  intros Hij.
+  rewrite loop_rename_internal.
+  rewrite <- compose_ktree_assoc.
+  rewrite cat_tensor.
+  rewrite Hij.
+  rewrite id_ktree_left.
+  rewrite tensor_id.
+  rewrite id_ktree_left.
+  reflexivity.
+Qed.
+
+End TraceLaws.
+
+Hint Rewrite @compose_ktree_assoc : lift_ktree.
+Hint Rewrite @tensor_id_lift : lift_ktree.
+Hint Rewrite @tensor_lift_id : lift_ktree.
+Hint Rewrite @lift_sum_elim : lift_ktree.
+
+(* Here we show that we can implement [ITree.cat] using
+   [tensor_ktree], [loop], and composition with the monoidal
+   natural isomorphisms. *)
+Section CatFromLoop.
+
+Variable E : Type -> Type.
+
+Theorem cat_from_loop {A B C} (ab : ktree E A B) (bc : ktree E B C) :
+  loop (sym_ktree >=> ab ⊗ bc) ⩯ ab >=> bc.
+Proof.
+  rewrite tensor_ktree_slide.
+  rewrite <- compose_ktree_assoc.
+  rewrite loop_compose.
+  rewrite tensor_swap.
+  repeat rewrite <- compose_ktree_assoc.
+  rewrite sym_nilpotent, id_ktree_left.
+  rewrite compose_loop.
+  erewrite yanking_ktree.
+  rewrite id_ktree_right.
+  reflexivity.
+Qed.
+
+End CatFromLoop.
