theories/Effects/StateFacts.v
@@ -13,6 +13,8 @@ From Paco Require Import paco.
 From ITree Require Import
      Basics.Basics
      Core.ITree
+     Core.KTree
+     Core.KTreeFacts
      Eq.UpToTaus
      Indexed.Sum
      Interp.Interp
