theories/ITree.v
@@ -1,6 +1,7 @@
 From ITree Require Export
      Basics.Basics
      Core.ITree
+     Core.KTree
      Eq.Eq
      Eq.UpToTaus
      Eq.SimUpToTaus
